src/Op.v
@@ -8,8 +8,8 @@ Definition eval_binop{w: nat}(op: binop)(v1 v2: word w): word w :=
   | OPlus => v1 ^+ v2
   | OMinus => v1 ^- v2
   | OTimes => v1 ^* v2
-  | OEq => if weq v1 v2 then wone w else wzero w
-  | OLt => if wlt_dec v1 v2 then wone w else wzero w
+  | OEq => if weq v1 v2 then $1 else $0
+  | OLt => if wlt_dec v1 v2 then $1 else $0
   | OAnd => v1 ^& v2
   end.
 
